Leanr.lean
@@ -15,6 +15,7 @@ import Leanr.OptimizerPasses.Rewrite
 import Leanr.OptimizerPasses.ConstantFold
 import Leanr.OptimizerPasses.ConstantSubst
 import Leanr.OptimizerPasses.TrivialConstraint
+import Leanr.OptimizerPasses.ZeroMultBus
 import Leanr.Optimizer
 import Leanr.Legacy.StringParser
 import Leanr.Legacy.OpenVM
